test/SDK/Keyring/MultiKeyring.dfy
@@ -1,0 +1,99 @@
+// RUN: %dafny /out:Output/MultiKeyring.exe "./MultiKeyring.dfy" ../../../src/extern/dotnet/UTF8.cs ../../../src/extern/dotnet/Random.cs ../../../src/extern/dotnet/AESEncryption.cs ../%bclib /compile:2
+// RUN: cp ../%bclib Output/
+// RUN: %mono ./Output/MultiKeyring.exe > "%t"
+// RUN: %diff "%s.expect" "%t"
+
+include "../../../src/SDK/Keyring/MultiKeyring.dfy"
+include "../../../src/SDK/Keyring/RawAESKeyring.dfy"
+include "../../../src/SDK/AlgorithmSuite.dfy"
+include "../../../src/Crypto/EncryptionSuites.dfy"
+include "../../../src/StandardLibrary/StandardLibrary.dfy"
+include "../../../src/StandardLibrary/UInt.dfy"
+include "../../../src/Util/UTF8.dfy"
+
+module TestRSAKeyring {
+  import opened StandardLibrary
+  import opened UInt = StandardLibrary.UInt
+  import RawAESKeyring
+  import EncryptionSuites
+  import MultiKeyringDef
+  import AlgorithmSuite
+  import UTF8
+
+  const name := UTF8.Encode("test Name").value;
+  const namespace := UTF8.Encode("test Namespace").value;
+
+  method TestOnEncryptOnDecryptWithGenerator() {
+    // TODO: mock children keyrings
+    var keyA, valA := UTF8.Encode("keyA").value, UTF8.Encode("valA").value;
+    var encryptionContext := [(keyA, valA)];
+    var child1Keyring := new RawAESKeyring.RawAESKeyring(UTF8.Encode("child1 Name").value, UTF8.Encode("child1 Namespace").value, seq(32, i => 0), EncryptionSuites.AES_GCM_256);
+    var child2Keyring := new RawAESKeyring.RawAESKeyring(UTF8.Encode("child2 Name").value, UTF8.Encode("child2 Namespace").value, seq(32, i => 0), EncryptionSuites.AES_GCM_256);
+    var keyIDs := new [][child2Keyring];
+    var multiKeyring := new MultiKeyringDef.MultiKeyring(child1Keyring, keyIDs);
+
+    var res := multiKeyring.OnEncrypt(AlgorithmSuite.AES_256_GCM_IV12_TAG16_HKDF_SHA384_ECDSA_P384, encryptionContext, None);
+    if onEncryptResult.Failure? || onEncryptResult.value.None? || |onEncryptResult.value.get.encryptedDataKeys| != 2 {
+      print "NOT CORRECT\n";
+      return;
+    }
+
+    var pdk := onEncryptResult.value.get.plaintextDataKey;
+    var edk1 := onEncryptResult.value.get.encryptedDataKeys[0];
+    var edk2 := onEncryptResult.value.get.encryptedDataKeys[1];
+
+    var res := multiKeyring.OnDecrypt(AlgorithmSuite.AES_256_GCM_IV12_TAG16_HKDF_SHA384_ECDSA_P384, encryptionContext, [edk1]);
+    if res.Success? && res.value.Some? && res.value.get.plaintextDataKey == pdk {
+      print "CORRECT\n";
+    } else {
+      print "NOT CORRECT\n";
+    }
+
+    res := multiKeyring.OnDecrypt(AlgorithmSuite.AES_256_GCM_IV12_TAG16_HKDF_SHA384_ECDSA_P384, encryptionContext, [edk2]);
+    if res.Success? && res.value.Some? && res.value.get.plaintextDataKey == pdk {
+      print "CORRECT\n";
+    } else {
+      print "NOT CORRECT\n";
+    }
+  }
+
+  method TestOnEncryptOnDecryptWithoutGenerator() {
+    // TODO: mock children keyrings and move encrypt <-> decrypt test into new test
+    var keyA, valA := UTF8.Encode("keyA").value, UTF8.Encode("valA").value;
+    var encryptionContext := [(keyA, valA)];
+    var child1Keyring := new RawAESKeyring.RawAESKeyring(UTF8.Encode("child1 Name").value, UTF8.Encode("child1 Namespace").value, seq(32, i => 0), EncryptionSuites.AES_GCM_256);
+    var child2Keyring := new RawAESKeyring.RawAESKeyring(UTF8.Encode("child2 Name").value, UTF8.Encode("child2 Namespace").value, seq(32, i => 0), EncryptionSuites.AES_GCM_256);
+    var keyIDs := new [][child1Keyring, child2Keyring];
+    var multiKeyring := new MultiKeyringDef.MultiKeyring(null, keyIDs);
+
+    var pdk := seq(32, i => 0);
+
+    var onEncryptResult := multiKeyring.OnEncrypt(AlgorithmSuite.AES_256_GCM_IV12_TAG16_HKDF_SHA384_ECDSA_P384, encryptionContext, Some(pdk));
+    if onEncryptResult.Failure? || onEncryptResult.value.None? || |onEncryptResult.value.get.encryptedDataKeys| != 2 {
+      print "NOT CORRECT\n";
+      return;
+    }
+
+    var edk1 := onEncryptResult.value.get.encryptedDataKeys[0];
+    var edk2 := onEncryptResult.value.get.encryptedDataKeys[1];
+
+    var res := multiKeyring.OnDecrypt(AlgorithmSuite.AES_256_GCM_IV12_TAG16_HKDF_SHA384_ECDSA_P384, encryptionContext, [edk1]);
+    if res.Success? && res.value.Some? && res.value.get.plaintextDataKey == pdk {
+      print "CORRECT\n";
+    } else {
+      print "NOT CORRECT\n";
+    }
+
+    res := multiKeyring.OnDecrypt(AlgorithmSuite.AES_256_GCM_IV12_TAG16_HKDF_SHA384_ECDSA_P384, encryptionContext, [edk2]);
+    if res.Success? && res.value.Some? && res.value.get.plaintextDataKey == pdk {
+      print "CORRECT\n";
+    } else {
+      print "NOT CORRECT\n";
+    }
+  }
+
+  method Main() {
+    TestOnEncryptOnDecryptWithGenerator();
+    TestOnEncryptOnDecryptWithoutGenerator();
+  }
+}
